DenotSem/Values.thy
@@ -1,10 +1,11 @@
 theory Values
-  imports Main IntersectionTypes
+  imports Main IntersectionTypes Consistency
 begin
 
 section "Values"
 
-datatype val = VNat nat | VFun func and
+
+(*datatype val = VNat nat | VFun func and
   func = VArrow val val (infix "\<mapsto>" 60) | VUnion func func (infix "\<squnion>" 59)
 
 fun v2t :: "val \<Rightarrow> ty" and f2t :: "func \<Rightarrow> ty" where
@@ -12,13 +13,20 @@ fun v2t :: "val \<Rightarrow> ty" and f2t :: "func \<Rightarrow> ty" where
   "v2t (VFun f) = f2t f" |
   "f2t (VArrow v1 v2) = (v2t v1) \<rightarrow> (v2t v2)" |
   "f2t (VUnion f1 f2) = (f2t f1) \<sqinter> (f2t f2)" 
-  
-fun le_val :: "val \<Rightarrow> val \<Rightarrow> bool" (infix "\<sqsubseteq>" 55) where
-  "(VNat n1) \<sqsubseteq> (VNat n2) = (n1 = n2)" |
-  "(VNat n1) \<sqsubseteq> (VFun f2) = False" |
-  "(VFun f1) \<sqsubseteq> (VNat n2) = False" |
-  "(VFun f1) \<sqsubseteq> (VFun f2) = f2t f2 <: f2t f1"
 
+abbreviation fun_app :: "func \<Rightarrow> val \<Rightarrow> val set" (infix "\<bullet>" 80) where
+  "f \<bullet> v \<equiv> {v'. f2t f <: v2t v \<rightarrow> v2t v' }"
   
-  
+abbreviation is_fun :: "func \<Rightarrow> bool" where
+  "is_fun f \<equiv> wf_ty (f2t f)"  
+
+abbreviation val_consis :: "val \<Rightarrow> val \<Rightarrow> bool" (infix "~" 55) where
+  "v1 ~ v2 \<equiv> v2t v1 ~ v2t v2"
+*)
+(*  
+fun join :: "val \<Rightarrow> val \<Rightarrow> val" (infix "\<squnion>" 59) where
+  "join (VNat n1) (VNat n2) = (if n1 = n2 then VNat n1 else undefined)" |
+  "join (VFun f1) (VFun f2) = VFun (f1 \<squnion> f2)"
+*)
+
 end
