DenotSem/Denot.thy
@@ -2,18 +2,20 @@ theory Denot
   imports Values Lambda Consistency
 begin
 
-fun E :: "exp \<Rightarrow> val list \<Rightarrow> val set" ("\<lbrakk>_\<rbrakk>_" [999] 1000) and
-    F :: "val \<Rightarrow> exp \<Rightarrow> val list \<Rightarrow> bool" where
-  Enat: "\<lbrakk>ENat n\<rbrakk> \<rho> = { VNat n }" |
+abbreviation fun_app :: "ty \<Rightarrow> ty \<Rightarrow> ty set" (infix "\<bullet>" 80) where
+  "f \<bullet> v \<equiv> {v'. f <: v \<rightarrow> v' }"
+
+fun E :: "exp \<Rightarrow> ty list \<Rightarrow> ty set" ("\<lbrakk>_\<rbrakk>_" [999] 1000) and
+    F :: "ty \<Rightarrow> exp \<Rightarrow> ty list \<Rightarrow> bool" where
+  Enat: "\<lbrakk>ENat n\<rbrakk> \<rho> = { TNat n }" |
   Evar: "\<lbrakk>EVar k\<rbrakk> \<rho> = (if k < length \<rho> then {\<rho>!k} else {})" |
-  Elam: "\<lbrakk>ELam e\<rbrakk> \<rho> = { t. is_val t \<and> F t e \<rho> }" |
-  Eapp: "\<lbrakk>EApp e1 e2\<rbrakk> \<rho> = { v'. \<exists> f v. f \<in> \<lbrakk>e1\<rbrakk>\<rho> \<and> v \<in> \<lbrakk>e2\<rbrakk>\<rho> \<and> v\<mapsto>v' \<sqsubseteq> f }" | 
-  Eprim: "\<lbrakk>EPrim f e1 e2\<rbrakk> \<rho> = { v. \<exists> n1 n2. VNat n1 \<in> \<lbrakk>e1\<rbrakk>\<rho> 
-          \<and> VNat n2 \<in> \<lbrakk>e2\<rbrakk>\<rho> \<and> v = VNat (f n1 n2) }" |
-  Eif: "\<lbrakk>EIf e1 e2 e3\<rbrakk> \<rho> = { v. \<exists> n. VNat n \<in> \<lbrakk>e1\<rbrakk>\<rho>
+  Elam: "\<lbrakk>ELam e\<rbrakk> \<rho> = { f. wf_fun f \<and> F f e \<rho> }" |
+  Eapp: "\<lbrakk>EApp e1 e2\<rbrakk> \<rho> = { v'. \<exists> f v. f \<in> \<lbrakk>e1\<rbrakk>\<rho> \<and> v \<in> \<lbrakk>e2\<rbrakk>\<rho> \<and> v' \<in> f \<bullet> v }" | 
+  Eprim: "\<lbrakk>EPrim f e1 e2\<rbrakk> \<rho> = { v. \<exists> n1 n2. TNat n1 \<in> \<lbrakk>e1\<rbrakk>\<rho> 
+          \<and> TNat n2 \<in> \<lbrakk>e2\<rbrakk>\<rho> \<and> v = TNat (f n1 n2) }" |
+  Eif: "\<lbrakk>EIf e1 e2 e3\<rbrakk> \<rho> = { v. \<exists> n. TNat n \<in> \<lbrakk>e1\<rbrakk>\<rho>
          \<and> (n = 0 \<longrightarrow> v \<in> \<lbrakk>e3\<rbrakk>\<rho>) \<and> (n \<noteq> 0 \<longrightarrow> v \<in> \<lbrakk>e2\<rbrakk>\<rho>) }" |
-  FNat : "F (VNat n) e \<rho> = False" | 
-  FFun: "F (v \<mapsto> v') e \<rho> = (v' \<in> \<lbrakk>e\<rbrakk>(v#\<rho>))" |
-  FUnion: "F (v1 \<squnion> v2) e \<rho> = (F v1 e \<rho> \<and> F v2 e \<rho>)"
+  FFun: "F (v \<rightarrow> v') e \<rho> = (v' \<in> \<lbrakk>e\<rbrakk>(v#\<rho>))" |
+  FUnion: "F (v1 \<sqinter> v2) e \<rho> = (F v1 e \<rho> \<and> F v2 e \<rho>)"
 
 end
