DenotSem/Deterministic.thy
@@ -1,109 +1,84 @@
 theory Deterministic
-  imports Values Denot Subsumption
+  imports Consistency Denot
 begin
 
+lemma merge_inter: "A ~ B \<Longrightarrow> merge A B \<approx> A \<sqinter> B"
+  apply (case_tac A)
+    apply (case_tac B)
+      apply force
+     apply simp
+  apply simp
+  apply (case_tac B)
+     apply simp
+    apply simp
+   apply simp
+    apply simp
+  done
+  
+lemma consistent_app: "\<lbrakk> f1 ~ f2; v1 ~ v2; v1' \<in> f1 \<bullet> v1; v2' \<in> f2 \<bullet> v2 \<rbrakk> \<Longrightarrow> v1' ~ v2'"
+  apply simp
+  sorry
+  
+lemma merge_app: assumes f1_v1: "v1' \<in> f1 \<bullet> v1" and f2_v2: "v2' \<in> f2 \<bullet> v2" and 
+  f1_f2: "f1 ~ f2" and v1_v2: "v1 ~ v2" and v1p_v2p: "v1' ~ v2'"
+  shows "merge v1' v2' \<in> merge f1 f2 \<bullet> merge v1 v2"
+proof -
+  have f1_v1p: "f1 <: v1 \<rightarrow> v1'" using f1_v1 by simp
+  have f2_v2p: "f2 <: v2 \<rightarrow> v2'" using f2_v2 by simp  
+  have "merge f1 f2 <: f1 \<sqinter> f2" using merge_inter f1_f2 ty_equiv_def by auto
+  also have "f1 \<sqinter> f2 <: (v1\<rightarrow>v1') \<sqinter> (v2\<rightarrow>v2')" using f1_v1p f2_v2p by (rule sub_mon)
+  also have "(v1 \<rightarrow> v1') \<sqinter> (v2 \<rightarrow> v2') <: (v1 \<sqinter> v2) \<rightarrow> (v1' \<sqinter> v2')" by (rule sub_dist_union_fun)
+  also have "... <: (merge v1 v2) \<rightarrow> (merge v1' v2')" apply (rule sub_arrow)
+      using merge_inter v1_v2 v1p_v2p ty_equiv_def apply auto done
+  finally  have "merge f1 f2 <: (merge v1 v2) \<rightarrow> (merge v1' v2')" using sub_trans by auto
+  then show ?thesis by simp
+qed
+    
 theorem deterministic:
-  "\<lbrakk> v1 \<in> E e \<rho>1; v2 \<in> E e \<rho>2; val_env \<rho>1; val_env \<rho>2; consis_env \<rho>1 \<rho>2 \<rbrakk>
-   \<Longrightarrow> v1 ~ v2 \<and> (\<exists> v12 \<rho>3. v1 \<squnion> v2 = v12 \<and> is_val v12 \<and> \<rho>1 \<squnion> \<rho>2 = \<rho>3 \<and> val_env \<rho>3 \<and> v12 \<in> \<lbrakk>e\<rbrakk>\<rho>3)"
+  "\<lbrakk> v1 \<in> E e \<rho>1; v2 \<in> E e \<rho>2; wf_env \<rho>1; wf_env \<rho>2; consis_env \<rho>1 \<rho>2 \<rbrakk>
+   \<Longrightarrow> v1 ~ v2 \<and> merge v1 v2 \<in> \<lbrakk>e\<rbrakk>(\<rho>1 \<sqinter> \<rho>2)"
 proof (induction e arbitrary: v1 v2 \<rho>1 \<rho>2)
   case (EVar x)
   have xr1: "x < length \<rho>1" using EVar(1) by (case_tac "x < length \<rho>1") auto
   have xr2: "x < length \<rho>2" using EVar(2) by (case_tac "x < length \<rho>2") auto
-  have v1_r1x: "v1 \<sqsubseteq> \<rho>1!x" using EVar(1) xr1 by auto
-  have v2_r2x: "v2 \<sqsubseteq> \<rho>2!x" using EVar(2) EVar(5) xr2 by auto
-  have v1_v2: "v1 ~ v2" using EVar lookup_consis apply auto
-    apply (case_tac "x < length \<rho>1") apply auto apply (case_tac "x < length \<rho>2") apply auto
-    apply (subgoal_tac "\<rho>1!x ~ \<rho>2!x") prefer 2 apply fastforce using consis_le by auto
-  have v_v1: "is_val v1" using EVar.prems(1) EVar.prems(3) is_val_sem by blast
-  have v_v2: "is_val v2" using EVar.prems(2) EVar.prems(4) is_val_sem by blast
-  obtain v12 where v12: "v1 \<squnion> v2 = Some v12" and v_v12: "is_val v12"
-    using v1_v2 v_v1 v_v2 consis_join_val by blast
-  obtain \<rho>3 where r123: "\<rho>1 \<squnion> \<rho>2 = Some \<rho>3" and v_r3: "val_env \<rho>3" 
-    using EVar consis_env_join by blast
-  have r3x: "\<rho>1!x \<squnion> \<rho>2!x = Some (\<rho>3!x)" using r123 xr1 join_env_nth consis_env_length 
-    using EVar.prems(5) by blast
-  have v12_r3: "v12 \<sqsubseteq> \<rho>3!x" using v1_r1x r123 r3x using mon v12 v2_r2x by blast
-  have xr3: "x < length \<rho>3" using join_env_length xr1 r123 consis_env_length EVar(5) by simp
-  have v12_e: "v12 \<in> \<lbrakk>EVar x\<rbrakk>\<rho>3" using v12_r3 xr3 v_v12 by simp
-  show ?case using v1_v2 v12 v_v12 r123 v12_e v_r3 by blast
+  have v1: "v1 = \<rho>1!x" using xr1 EVar(1) by auto
+  have v2: "v2 = \<rho>2!x" using xr2 EVar(2) by auto
+  have v1_v2: "v1 ~ v2" using EVar xr1 xr2 by auto 
+  have v_v1: "wf_ty v1" using EVar(1) EVar(3) xr1 by auto
+  have v_v2: "wf_ty v2" using EVar(2) EVar(4) xr2 by auto
+  have r3x: "merge v1 v2 = (\<rho>1 \<sqinter> \<rho>2)!x" 
+    using v1 v2 consis_env_inter[of \<rho>1 \<rho>2 x] EVar(5) xr1 by simp
+  have xr3: "x < length (\<rho>1 \<sqinter> \<rho>2)" using inter_env_length xr1 EVar(5) by simp
+  have v12_e: "merge v1 v2 \<in> \<lbrakk>EVar x\<rbrakk>(\<rho>1 \<sqinter> \<rho>2)" using r3x xr3 by simp
+  show ?case using v1_v2 v12_e by simp
 next
-  case (ENat x)
-  obtain \<rho>3 where r123: "\<rho>1 \<squnion> \<rho>2 = Some \<rho>3" and v_r3: "val_env \<rho>3" 
-    using ENat consis_env_join by blast
-  show ?case using ENat r123 v_r3 by auto 
+  case (ENat n)
+  have v1: "v1 = TNat n" using ENat(1) by simp
+  have v2: "v2 = TNat n" using ENat(2) by simp
+  have m: "merge v1 v2 = TNat n" using v1 v2 by simp
+  show ?case using m v1 v2 by simp
 next
   case (ELam e)
   then show ?case sorry
 next
-  case (EApp e1 e2)
-  obtain f1 v21 where v_v1: "is_val v1" and f1_e1: "VFun f1 \<in> \<lbrakk>e1\<rbrakk>\<rho>1" and
-    v21_e2: "v21 \<in> \<lbrakk>e2\<rbrakk>\<rho>1" and v21v1_f1: "[(v21, v1)] \<sqsubseteq> f1" using EApp.prems(1) by auto
-  obtain f2 v22 where v_v2: "is_val v2" and f2_e1: "VFun f2 \<in> \<lbrakk>e1\<rbrakk>\<rho>2" and
-    v22_e2: "v22 \<in> \<lbrakk>e2\<rbrakk>\<rho>2" and v22v2_f2: "[(v22, v2)] \<sqsubseteq> f2" using EApp.prems(2) by auto
-  have f1_f2: "VFun f1 ~ VFun f2"
-    using EApp.IH(1) EApp.prems(3) EApp.prems(4) EApp.prems(5) f1_e1 f2_e1 by blast
-  have cf12: "VFun f1 ~ VFun f2" using EApp.IH(1)[of "VFun f1" \<rho>1 "VFun f2"] f1_f2 by blast
-  obtain vf12 \<rho>3 where
-    f12_vf12: "VFun f1 \<squnion> VFun f2 = Some vf12" and 
-    v_vf12: "is_val vf12" and r12_r3: "\<rho>1 \<squnion> \<rho>2 = Some \<rho>3" and v_r3: "val_env \<rho>3" and
-    vf12_e1: "vf12 \<in> \<lbrakk>e1\<rbrakk>\<rho>3" using EApp.IH(1)[of "VFun f1" \<rho>1 "VFun f2" \<rho>2] EApp.prems(3) 
-      EApp.prems(4) EApp.prems(5) f1_e1 f2_e1 by blast 
-  obtain v12 \<rho>3' where v21_v22: "v21 ~ v22" and
-    v21_v22_v12: "v21 \<squnion> v22 = Some v12" and v_v12: "is_val v12" and
-    r12_r3p: "\<rho>1 \<squnion> \<rho>2 = Some \<rho>3'" and v_r3p: "val_env \<rho>3'" and v12_e2: "v12 \<in> \<lbrakk>e2\<rbrakk>\<rho>3"
-    using EApp.IH(2) v21_e2 v22_e2 EApp.prems(3) EApp.prems(4) EApp.prems(5)
-    by (metis  option.inject r12_r3)
-  obtain v21' v1' where v21p_f1: "(v21',v1') \<in> set f1" and 
-    v21p_v21: "v21' \<sqsubseteq> v21" and v1_v1p: "v1 \<sqsubseteq> v1'"
-    sorry
-    (*using v21v1_f1
-    by (meson le_fun_sub_pair list.set_intros(1))
-      *)
-  obtain v22' v2' where v22p_f2: "(v22',v2') \<in> set f2" and 
-    v22p_v22: "v22' \<sqsubseteq> v22" and v2_v2p: "v2 \<sqsubseteq> v2'"
-    sorry
-    (*using v22v2_f2
-    by (meson le_fun_sub_pair list.set_intros(1))*)
-  from f1_f2 v21p_f1 v22p_f2 have 1: "(v21' ~ v22' \<and> v1' ~ v2') \<or> \<not> v21' ~ v22'" 
-    using consis_inconsis_sym by blast
-  have c_v1v2: "v1 ~ v2"
-    using 1 consis_le_inconsis_le v1_v1p v21_v22 v21p_v21 v22p_v22 v2_v2p by blast
-  obtain v3 where v1_v2_v3: "v1 \<squnion> v2 = Some v3" and v_v3: "is_val v3" 
-    using c_v1v2 consis_join_val v_v1 v_v2 by auto
-  have "[(v12, v3)] \<sqsubseteq> f1 @ f2" 
-  proof -
-    have 1: "[(v21',v1'),(v22',v2')] \<sqsubseteq> f1@f2" 
-      apply (rule le_fun_subset) apply (rule subsetI) using v21p_f1 v22p_f2 apply force done
-    have v21p_v22p: "v21' ~ v22'" using v21_v22 v21p_v21 v22p_v22 consis_le by blast
-    obtain w2 where w2: "v21' \<squnion> v22' = Some w2" and v_w2: "is_val w2" 
-      using v21p_v22p consis_join_val[of v21' v22'] EApp.prems(3) EApp.prems(4)
-        f1_e1 f2_e1 is_val_sem v21p_f1 v22p_f2 by blast
-    have 2: "[(v12,v3)] \<sqsubseteq> [(v21',v1'),(v22',v2')]"
-    proof -
-      have a: "[(v12,v3)] \<sqsubseteq> [(v12,v1),(v12,v2)]"
-        using v1_v2_v3 by (rule le_distr)
-      have b: "[(v12,v1),(v12,v2)] \<sqsubseteq> [(v21',v1'),(v22',v2')]"
-        apply (rule le_cons_left) prefer 3 apply force
-         apply (rule le_cons_right1) apply (rule le_arrow)
-        using Values.le_trans le_join_left v21_v22_v12 v21p_v21 apply blast
-        using v1_v1p apply blast
-         apply blast
-        apply (rule le_cons_right2)
-        apply (rule le_arrow)
-        using le_trans le_join_right v21_v22_v12 v22p_v22 apply blast
-        using v2_v2p apply blast
-        done
-      show ?thesis using a b le_fun_trans by meson
-    qed
-    show ?thesis using 2 1 le_fun_trans by meson
-  qed
-  then have 2: "v3 \<in> \<lbrakk>EApp e1 e2\<rbrakk>\<rho>3" using v_v3 vf12_e1 vf12_e1 f12_vf12 v12_e2 apply simp
-    apply (rule_tac x="f1@f2" in exI) apply simp
-    apply (rule_tac x=v12 in exI) apply simp done
-  show ?case using "2" \<open>v1 \<squnion> v2 = Some v3\<close> c_v1v2 r12_r3 v_r3 v_v3 by blast
+  case (EApp e1 e2 v1' v2')
+  obtain f1 v1 where f1_e1: "f1 \<in> \<lbrakk>e1\<rbrakk>\<rho>1" and v1_e2: "v1 \<in> \<lbrakk>e2\<rbrakk>\<rho>1" and v1p_f1_v1: "v1' \<in> f1 \<bullet> v1"
+    using EApp(3) by auto
+  obtain f2 v2 where f2_e1: "f2 \<in> \<lbrakk>e1\<rbrakk>\<rho>2" and v2_e2: "v2 \<in> \<lbrakk>e2\<rbrakk>\<rho>2" and v2p_f2_v2: "v2' \<in> f2 \<bullet> v2"
+    using EApp(4) by auto
+  have f1_f2: "f1 ~ f2" using EApp.IH(1) f1_e1 f2_e1 EApp(5) EApp(6) EApp(7) by blast
+  have m_f1f2: "merge f1 f2 \<in> \<lbrakk>e1\<rbrakk>(\<rho>1\<sqinter>\<rho>2)" using EApp.IH(1) f1_e1 f2_e1 EApp(5) EApp(6) EApp(7) by blast
+  have v1_v2: "v1 ~ v2" using EApp.IH(2) v1_e2 v2_e2 EApp(5) EApp(6) EApp(7) by blast
+  have m_v12: "merge v1 v2 \<in> \<lbrakk>e2\<rbrakk>(\<rho>1\<sqinter>\<rho>2)" using EApp.IH(2) v1_e2 v2_e2 EApp(5) EApp(6) EApp(7) by blast
+  have v1p_v2p: "v1' ~ v2'" using f1_f2 v1_v2 v1p_f1_v1 v2p_f2_v2 consistent_app by blast
+  have m_v12p_f12_v12: "merge v1' v2' \<in> (merge f1 f2) \<bullet> (merge v1 v2)"
+    using v1p_f1_v1 v2p_f2_v2 f1_f2 v1_v2 v1p_v2p merge_app by blast
+  show ?case using v1p_v2p m_v12p_f12_v12 m_f1f2 m_v12 by auto
 next
   case (EPrim f e1 e2)
-  then show ?case sorry
+  then show ?case apply simp apply clarify apply simp apply (rule conjI) 
+      sorry
+      
 next
   case (EIf e1 e2 e3)
   then show ?case sorry
